src/Core.TypeCheck.fst
@@ -2,30 +2,66 @@ module Core.TypeCheck
 
 open Core.Fc
 open Core.Name
-open Core.Raw
 open Core.Ltt
 open Core.Tc
 open Core.Environment
+open Core.Context
+open Core.Weaken
+open Core.Evaluate
+
+module L = FStar.List.Tot
 
 (** A mapping of the in-scope names to the type that they
     are bound to. *)
-private type local_ctxt vars = local_env raw_term vars
+private type local_ctxt vars = local_env term vars
 
-//private val expand_binder : #vars:list local_name -> #
+private let assert_is_type
+  (#vars:list local_name)
+  (fl:fc)
+  (t:term vars)
+  : TcNull unit
+  = if Universe? t
+    then ()
+    else raise (TcTermIsNotAType fl t)
 
-private val lookup_ty : #vars:list local_name
-                      -> fc
-                      -> any_name
-                      -> local_ctxt vars
-                      -> TcNull (raw_term vars)
-let lookup_ty #vars fc n ctx =
-  let res = match n with
-    | LocalName ln ->
-      binder_ty (env_lookup raw_term ln ctx)
-    | _ -> None in
-  match res with
-  | Some v -> v
-  | None -> lookup' fc n
+val infer_type : #vars:list local_name
+               -> term vars
+               -> local_ctxt vars
+               -> TcNull (ty:term vars)
 
-//val infer_type : body:raw_term -> env:local_scope -> TcNull (ty:raw_term)
-//let infer_type body env =
+val check_type : #vars:list local_name
+               -> ty:term vars
+               -> t:term vars
+               -> local_ctxt vars
+               -> TcNull (ty:term vars)
+
+let rec infer_type #vars target envr =
+  match target with
+  // T-Var
+  | Local _ bv -> local_env_lookup_ty term bv envr
+  // T-Var
+  | Ref fc gn ->
+    let gdef: global_def = lookup' fc (GlobalName gn) in
+    L.append_l_nil vars;
+    weaken_ns term vars gdef.type'
+  // T-Type
+  | Universe _ -> Universe EmptyFc
+  // T-Pi
+  | Abs fc n (Pi tyA) tyB ->
+    assert_is_type fc (infer_type tyA envr);
+    let envr' = ConsEnv (Pi tyA) n envr in
+    assert_is_type fc (infer_type tyB envr');
+    Universe EmptyFc
+  // T-Lam
+  | Abs fc n (Lam tyS) body ->
+    let envr' = ConsEnv (Lam tyS) n envr in
+    let tyT = infer_type body envr' in
+    assert_is_type fc tyS;
+    Abs EmptyFc n (Pi tyS) tyT
+  // T-Let
+  | Abs fc n (Let e1 tyS) e2 ->
+
+and check_type #vars ty t envr =
+
+type typed_term (vars:list local_name) =
+  | Typed : value:term vars -> ty:term vars{ty == infer_type value} -> typed_term vars
