TODO.md
@@ -1,13 +1,17 @@
 # TODO
-* Implement typecheck
-* Write down what the type theory is
-* Refactor the `total_ordering` stuff out of `Core.Name` and
+- [x] Write down what the type theory is
+- [ ] Implement typecheck
+  1. Write function to convert `raw_term` to `term`
+  2. Implement typechecker on `term`
+
+
+- [ ]  Refactor the `total_ordering` stuff out of `Core.Name` and
   into something like `Util.TotalOrdering`. Define a typeclass
   that indicates that there is a total ordering on a type and
   define variants of `ordmap` and `ordset` that just take a key
   type (that has to have an instance of the typeclass) and a
   value type.
-* Implement elaboration monad
+- [ ] Implement elaboration monad
   1. Develop list of elaboration monad tactics
   2. Implement skeleton of the elaboration monad
   3. Implement elaboration monad tactics (add each tactic below)
